

## Conversion between weight and length

In mizer we have the following PDE for a density  $N(w)$  in a variable  $w$ :

$$\partial N / \partial t = -\partial J_w / \partial w - mw(n-1)N$$

where

$$J_w = (Aw^n - Bw)N - Dw^{n+1}\partial N / \partial w.$$

We want to convert this into a PDE for a density  $u(l, t)$  in a variable  $l$  related to  $w$  by  $w = al^b$  where  $n = 1 - 1/b$ . Write the PDE in the form

$$\partial u / \partial t = -\partial J_l / \partial l - m/lu$$

where

$$J_l = k(L_\infty^0 - l)u - \alpha l \partial u / \partial l.$$

We would like to express the parameters  $k$ ,  $L_\infty^0$  and  $\alpha$  in terms of the parameters  $A$ ,  $B$  and  $D$ .

### Step 1: Relate the Densities using Conservation

The number of particles must be conserved under the change of variables. This means that the number of particles in an infinitesimal interval  $dw$  must be equal to the number of particles in the corresponding interval  $dl$ .

$$N(w, t)dw = u(l, t)dl$$

This gives the relationship between the two densities:

$$u(l, t) = N(w, t) \frac{dw}{dl}$$

Given the transformation  $w = al^b$ , we can calculate the derivative  $\frac{dw}{dl}$ :

$$\frac{dw}{dl} = abl^{b-1}$$

Substituting this into the relation between the densities, we get:

$$u(l, t) = N(w(l), t) \cdot (abl^{b-1})$$

From this, we can express  $N(w, t)$  in terms of  $u(l, t)$ :

$$N(w, t) = \frac{u(l, t)}{abl^{b-1}}$$

## Step 2: Transform the PDE

The original PDE is:

$$\frac{\partial N}{\partial t} = -\frac{\partial J_w}{\partial w} - mw^{n-1}N$$

We can write this in conservation form:

$$\frac{\partial N}{\partial t} + \frac{\partial J_w}{\partial w} = -mw^{n-1}N$$

To change variables from  $(w, t)$  to  $(l, t)$ , we multiply the entire equation by  $\frac{dw}{dl}$ :

$$\frac{\partial N}{\partial t} \frac{dw}{dl} + \frac{\partial J_w}{\partial w} \frac{dw}{dl} = -mw^{n-1}N \frac{dw}{dl}$$

Let's transform each term:

- **Time derivative term:**

$$\frac{\partial N}{\partial t} \frac{dw}{dl} = \frac{\partial}{\partial t} \left( N \frac{dw}{dl} \right) - N \frac{\partial}{\partial t} \left( \frac{dw}{dl} \right)$$

Since  $\frac{dw}{dl} = abl^{b-1}$  does not depend on time  $t$ , the second term is zero. Thus:

$$\frac{\partial N}{\partial t} \frac{dw}{dl} = \frac{\partial}{\partial t} \left( N \frac{dw}{dl} \right) = \frac{\partial u}{\partial t}$$

- **Flux derivative term:** Using the chain rule:

$$\frac{\partial J_w}{\partial w} \frac{dw}{dl} = \frac{\partial J_w}{\partial l}$$

- **Source term:**

$$-mw^{n-1}N \frac{dw}{dl} = -mw^{n-1}u$$

We use the given relations  $w = al^b$  and  $n = 1 - 1/b$ , which implies  $n - 1 = -1/b$ .

$$w^{n-1} = (al^b)^{n-1} = a^{n-1}l^{b(n-1)} = a^{-1/b}l^{-1}$$

So the source term becomes:

$$-ma^{-1/b}l^{-1}u = -\frac{ma^{-1/b}}{l}u$$

Substituting these transformed terms back into the PDE, we get:

$$\frac{\partial u}{\partial t} + \frac{\partial J_w}{\partial l} = -\frac{ma^{-1/b}}{l}u$$

Rearranging this gives:

$$\frac{\partial u}{\partial t} = -\frac{\partial J_w}{\partial l} - \frac{ma^{-1/b}}{l}u$$

This equation has the same form as the target equation if we identify  $J_l = J_w$  and if the parameter  $m$  in the target equation is understood as a new parameter  $m_{new} = m_{old}a^{-1/b}$ .

### Step 3: Transform the Flux $J_w$

Now, we express the flux  $J_w$  in terms of  $u$  and  $l$ . The expression for  $J_w$  is:

$$J_w = (Aw^n - Bw)N - Dw^{n+1} \frac{\partial N}{\partial w}$$

We need to substitute for  $w$ ,  $N$ , and  $\frac{\partial N}{\partial w}$ . First, let's find the derivative  $\frac{\partial N}{\partial w}$  in terms of  $u$  and  $l$ :

$$\begin{aligned} \frac{\partial N}{\partial w} &= \frac{dl}{dw} \frac{\partial N}{\partial l} = \frac{1}{abl^{b-1}} \frac{\partial}{\partial l} \left( \frac{u}{abl^{b-1}} \right) \\ \frac{\partial N}{\partial w} &= \frac{1}{abl^{b-1}} \left[ \frac{1}{abl^{b-1}} \frac{\partial u}{\partial l} - u \frac{(b-1)}{abl^b} \right] = \frac{1}{(ab)^2 l^{2b-2}} \frac{\partial u}{\partial l} - \frac{u(b-1)}{(ab)^2 l^{2b-1}} \end{aligned}$$

Now substitute this and the expressions for  $w$  and  $N$  into  $J_w$ :

- **First part of  $J_w$  (advection term):**

$$(Aw^n - Bw)N = (A(al^b)^n - B(al^b)) \frac{u}{abl^{b-1}}$$

Using  $n = 1 - 1/b \Leftrightarrow bn = b - 1$ :

$$(Aa^n l^{b-1} - Bal^b) \frac{u}{abl^{b-1}} = \left( \frac{Aa^{n-1}}{b} - \frac{B}{b} l \right) u$$

- **Second part of  $J_w$  (diffusion term):**

$$-Dw^{n+1} \frac{\partial N}{\partial w} = -D(al^b)^{n+1} \left[ \frac{1}{(ab)^2 l^{2b-2}} \frac{\partial u}{\partial l} - \frac{u(b-1)}{(ab)^2 l^{2b-1}} \right]$$

The exponent of  $l$  is  $b(n+1) = b(1 - 1/b + 1) = 2b - 1$ .

$$\begin{aligned} &-Da^{n+1} l^{2b-1} \left[ \frac{1}{a^2 b^2 l^{2b-2}} \frac{\partial u}{\partial l} - \frac{u(b-1)}{a^2 b^2 l^{2b-1}} \right] \\ &= -\frac{Da^{n-1}}{b^2} l \frac{\partial u}{\partial l} + \frac{Da^{n-1}(b-1)}{b^2} u \end{aligned}$$

Combining all parts of  $J_w$ :

$$J_w = \left( \frac{Aa^{n-1}}{b} + \frac{Da^{n-1}(b-1)}{b^2} \right) u - \frac{B}{b} lu - \frac{Da^{n-1}}{b^2} l \frac{\partial u}{\partial l}$$

### Step 4: Identify the Coefficients

We now have the transformed PDE:

$$\frac{\partial u}{\partial t} = -\frac{\partial J_w}{\partial l} - \dots$$

with  $J_w$  as derived above. We compare this flux with the target flux  $J_l$ :

$$J_l = k(L_\infty^0 - l)u - \alpha l \frac{\partial u}{\partial l} = (kL_\infty^0)u - klu - \alpha l \frac{\partial u}{\partial l}$$

By setting  $J_l = J_w$  and comparing the coefficients of the terms  $u$ ,  $lu$ , and  $l \frac{\partial u}{\partial l}$ , we find the expressions for  $k$ ,  $L_\infty^0$ , and  $\alpha$ .

- **Coefficient of  $l \frac{\partial u}{\partial l}$ :**

$$-\alpha = -\frac{Da^{n-1}}{b^2} \Leftrightarrow \alpha = \frac{Da^{n-1}}{b^2}$$

- **Coefficient of  $lu$ :**

$$-k = -\frac{B}{b} \Leftrightarrow k = \frac{B}{b}$$

- **Coefficient of  $u$ :**

$$\begin{aligned} kL_{\infty}^0 &= \frac{Aa^{n-1}}{b} + \frac{Da^{n-1}(b-1)}{b^2} \\ \Leftrightarrow L_{\infty}^0 &= \frac{1}{k} \left( \frac{Aa^{n-1}}{b} + \frac{Da^{n-1}(b-1)}{b^2} \right) = \frac{b}{B} a^{n-1} \left( \frac{A}{b} + \frac{D(b-1)}{b^2} \right) \\ \Leftrightarrow L_{\infty}^0 &= \frac{a^{n-1}}{B} \left( A + \frac{D(b-1)}{b} \right) \end{aligned}$$

### Final Expressions

The expressions for  $k$ ,  $L_{\infty}^0$ , and  $\alpha$  in terms of  $A$ ,  $B$ ,  $D$ , and the transformation parameters  $a$  and  $b$  are:

$$\begin{aligned} k &= \frac{B}{b}, \\ \alpha &= \frac{Da^{n-1}}{b^2}, \\ L_{\infty}^0 &= \frac{a^{n-1}}{B} \left( A + D \frac{b-1}{b} \right). \end{aligned}$$

These can also be expressed in terms of  $n$  by using the relations  $n = 1 - 1/b$ , which implies  $b = \frac{1}{1-n}$  and  $n - 1 = -1/b$ . Also, the term  $\frac{b-1}{b} = 1 - \frac{1}{b} = n$ .

Substituting these into the expressions gives:

$$\begin{aligned} k &= B(1-n), \\ \alpha &= Da^{-(1-n)}(1-n)^2, \\ L_{\infty}^0 &= \frac{a^{-(1-n)}}{B}(A + Dn). \end{aligned}$$

**Note:** The parameter  $L_{\infty}^0$  is related to the asymptotic length  $L_{\infty}$  in the expression for the average growth rate

$$g(l) = k(L_{\infty} - l)$$

by

$$L_{\infty} = L_{\infty}^0 + \frac{\alpha}{k}.$$

### Inverting the Relations

We will now solve express the parameters  $A$ ,  $B$ , and  $D$  in terms of  $k$ ,  $L_{\infty}^0$  and  $\alpha$ .

#### 1. Solving for $B$

From the first equation, we can directly isolate  $B$ :

$$\begin{aligned} k &= B(1-n) \\ \Leftrightarrow B &= \frac{k}{1-n} \end{aligned}$$

## 2. Solving for D

From the second equation, we can directly isolate  $D$ :

$$\begin{aligned}\alpha &= Da^{-(1-n)}(1-n)^2 \\ \Leftrightarrow D &= \frac{\alpha}{a^{-(1-n)}(1-n)^2} \\ \Leftrightarrow D &= \frac{\alpha a^{1-n}}{(1-n)^2}\end{aligned}$$

## 3. Solving for A

From the third equation, we can isolate  $A$ :

$$L_{\infty}^0 = \frac{a^{-(1-n)}}{B}(A + Dn)$$

Rearranging the terms to solve for  $A$ :

$$\begin{aligned}BL_{\infty}^0 &= a^{-(1-n)}(A + Dn), \\ \Leftrightarrow BL_{\infty}^0 a^{1-n} &= A + Dn, \\ \Leftrightarrow A &= BL_{\infty}^0 a^{1-n} - Dn.\end{aligned}$$

Now, we substitute the expressions we found for  $B$  and  $D$ :

$$A = \left(\frac{k}{1-n}\right)L_{\infty}^0 a^{1-n} - \left(\frac{\alpha a^{1-n}}{(1-n)^2}\right)n$$

We can factor out common terms to simplify the expression for  $A$ :

$$A = \frac{a^{1-n}}{(1-n)} \left( kL_{\infty}^0 - \frac{n\alpha}{1-n} \right)$$

## Final Inverted Relations

The final expressions for  $A$ ,  $B$ , and  $D$  are:

$$\begin{aligned}A &= \frac{a^{1-n}}{1-n} \left( kL_{\infty}^0 - \frac{n\alpha}{1-n} \right), \\ B &= \frac{k}{1-n}, \\ D &= \frac{\alpha a^{1-n}}{(1-n)^2}.\end{aligned}$$